Flow.v
@@ -1,0 +1,123 @@
+
+From Coq Require Import ZArith Lia Bool List String Program.Equality.
+From Coq Require Import FunctionalExtensionality PropExtensionality.
+From CDF Require Import Separation Seplog.
+
+Local Open Scope string_scope.
+Local Open Scope nat_scope.
+Local Open Scope list_scope.
+
+Section Flow.
+
+Definition flow : Type := heap -> heap -> Prop.
+
+Definition fexists {A: Type} (P: A -> flow) : flow :=
+  fun h1 h2 => exists a: A, P a h1 h2.
+
+(* Print assertion. *)
+Definition freq (P: precond) : flow :=
+  fun h1 h2 => exists h3 h4,
+    h1 = hunion h3 h4 /\ hdisjoint h3 h4 /\ P h3 /\ h2 = h4.
+    (* h3 is the part of the heap that is taken away by req,
+    h4 is what is left *)
+
+Definition fens (P: postcond) : flow :=
+  fun h1 h2 => exists h3,
+  exists r, (* TODO *)
+    P r h3 /\ h2 = hunion h1 h3 /\ hdisjoint h1 h3.
+
+Definition fempty : flow := fens (fun r h => True).
+
+Definition fseq (f1 f2 : flow) : flow :=
+  (* fun h1 h2 => exists h3, f1 h1 h3 /\ f2 h3 h2. *)
+  fun h1 h2 => exists h3, f1 h1 h3 -> f2 h3 h2.
+
+Infix ";;" := fseq (at level 80, right associativity).
+
+(* TODO disjunction *)
+
+(* TODO functions *)
+
+(* Definition fn (name : string) : flow :=
+  fun _ => True. *)
+
+(* forward rules. says how to produce a flow from a program *)
+Inductive forward : com -> flow -> Prop :=
+  | fw_skip:
+    forward SKIP fempty
+  | fw_pure: forall n,
+    forward (PURE n) (fens (fun res h => res = n))
+  | fw_get: forall l v, 
+    forward (GET l)
+      (freq (fun h => h = hsingle l v) ;;
+      fens (fun r h => h = hsingle l v /\ r = v))
+
+  (* | fw_set: forall f l v, *)
+    (* forward f (SET l v) f *)
+  (* | fw_let: forall f e1 e2, *)
+    (* forward f (LET e1 e2) f *)
+
+  .
+
+(* Example e1 : forall h1 h2, red (PURE 0, h1) (PURE 0, h2).
+intros.
+Qed. *)
+
+
+(* Inductive a : flow -> com -> flow -> Prop := . *)
+
+(* Inductive red: com * heap -> com * heap -> Prop := *)
+
+(* red is a small step relation, soundness eventually needs to be proved for star red *)
+
+Ltac inv H := inversion H; clear H; subst.
+
+Theorem soundness : forall f c1 c2 h1 h2,
+(* doesn't work for stuff that doesn't reduce, like pure *)
+  red (c1, h1) (c2, h2) ->
+  forward c1 f ->
+  f h1 h2.
+Proof.
+  intros f c1 c2 h1 h2 Hr Hf.
+  induction Hf.
+  - inv Hr.
+  - inv Hr.
+  -
+  (* inversion Hr. *)
+  (* assert (fh = fempty). *)
+  inv Hr.
+
+  (* assuming we start in state h2 *)
+  (* the intermediate states in sequencing are also h2 *)
+  unfold fseq.
+  (* exists h2. *)
+  (* intros hist. *)
+  exists (hfree l h2).
+
+  (* now partition the heap into h2 and emp,
+  and assume there is h2[l:=v] *)
+  unfold freq.
+  intros [h3 [h4 [Hu [Hd [Hg He]]]]].
+  subst.
+  (* h2 is now called h0, and h4 is empty *)
+
+  (* add another empty piece of heap, h3 *)
+  unfold fens.
+  exists (hsingle l v).
+  exists v.
+  subst.
+  split.
+  split; reflexivity.
+  split.
+  rewrite He.
+  rewrite hunion_comm.
+  reflexivity.
+  rewrite hdisjoint_sym; auto.
+  unfold hsingle in *.
+  pose proof hfree_hunion_hupdate as hh.
+  rewrite hfree_hunion_hupdate.
+  rewrite hdisjoint_sym; auto.
+  auto.
+Qed.
+
+End Flow.
